pcuic/PCUICtoTemplate.v
@@ -1,0 +1,96 @@
+From Coq Require Import Bool String List Program BinPos Compare_dec Omega.
+From MetaCoq.Template Require Import config utils AstUtils BasicAst Ast.
+From MetaCoq.Checker Require Import WfInv Typing Weakening TypingWf.
+From MetaCoq.PCUIC Require Import PCUICAst PCUICAstUtils PCUICInduction PCUICLiftSubst
+     PCUICUnivSubst PCUICTyping PCUICGeneration.
+Require Import String.
+Local Open Scope string_scope.
+Set Asymmetric Patterns.
+
+Module TC := Ast.
+Module P := PCUICAst.
+
+Fixpoint trans (t : P.term) : TC.term :=
+  match t with
+  | P.tRel n => TC.tRel n
+  | P.tVar n => TC.tVar n
+  | P.tEvar ev args => TC.tEvar ev (List.map trans args)
+  | P.tSort u => TC.tSort u
+  | P.tConst c u => TC.tConst c u
+  | P.tInd c u => TC.tInd c u
+  | P.tConstruct c k u => TC.tConstruct c k u
+  | P.tLambda na T M => TC.tLambda na (trans T) (trans M)
+  | P.tApp u v => TC.mkApps (trans u) [trans v]
+  | P.tProd na A B => TC.tProd na (trans A) (trans B)
+  | P.tLetIn na b t b' => TC.tLetIn na (trans b) (trans t) (trans b')
+  | P.tCase ind p c brs =>
+    let brs' := List.map (on_snd trans) brs in
+    TC.tCase ind (trans p) (trans c) brs'
+  | P.tProj p c => TC.tProj p (trans c)
+  | P.tFix mfix idx =>
+    let mfix' := List.map (map_def trans trans) mfix in
+    TC.tFix mfix' idx
+  | P.tCoFix mfix idx =>
+    let mfix' := List.map (map_def trans trans) mfix in
+    TC.tCoFix mfix' idx
+  end.
+
+Definition trans_decl (d : P.context_decl) :=
+  let 'P.Build_context_decl na b t := d in
+  {| TC.decl_name := na;
+     TC.decl_body := option_map trans b;
+     TC.decl_type := trans t |}.
+
+Definition trans_local Γ := List.map trans_decl Γ.
+
+Definition trans_one_ind_body (d : P.one_inductive_body) :=
+  {| TC.ind_name := d.(P.ind_name);
+     TC.ind_type := trans d.(P.ind_type);
+     TC.ind_kelim := d.(P.ind_kelim);
+     TC.ind_ctors := List.map (fun '(x, y, z) => (x, trans y, z)) d.(P.ind_ctors);
+     TC.ind_projs := List.map (fun '(x, y) => (x, trans y)) d.(P.ind_projs) |}.
+
+Definition trans_local_entry (le : P.local_entry) :=
+  match le with
+  | P.LocalDef ld => TC.LocalDef (trans ld)
+  | P.LocalAssum la => TC.LocalAssum (trans la)
+  end.
+
+Definition trans_one_ind_entry (d : P.one_inductive_entry) : TC.one_inductive_entry :=
+  {| TC.mind_entry_typename := d.(P.mind_entry_typename);
+     TC.mind_entry_arity := trans d.(P.mind_entry_arity);
+     TC.mind_entry_template := d.(P.mind_entry_template);
+     TC.mind_entry_consnames := d.(P.mind_entry_consnames);
+     TC.mind_entry_lc := map trans d.(P.mind_entry_lc) |}.
+
+Definition trans_minductive_entry (e : P.mutual_inductive_entry) :  TC.mutual_inductive_entry :=
+  {| TC.mind_entry_record := e.(P.mind_entry_record);
+     TC.mind_entry_finite := e.(P.mind_entry_finite);
+     TC.mind_entry_params := List.map (fun '(x, y) => (x, trans_local_entry y)) e.(P.mind_entry_params);
+     TC.mind_entry_inds := List.map trans_one_ind_entry e.(P.mind_entry_inds);
+     TC.mind_entry_universes := e.(P.mind_entry_universes);
+     TC.mind_entry_private := e.(P.mind_entry_private) |}.
+
+Definition trans_constant_body (bd : P.constant_body) : TC.constant_body :=
+  {| TC.cst_type := trans bd.(P.cst_type);
+     TC.cst_body := option_map trans bd.(P.cst_body);
+     TC.cst_universes := bd.(P.cst_universes) |}.
+
+Definition trans_minductive_body md :=
+  {| TC.ind_finite := md.(P.ind_finite);
+     TC.ind_npars := md.(P.ind_npars);
+     TC.ind_params := trans_local md.(P.ind_params);
+     TC.ind_bodies := map trans_one_ind_body md.(P.ind_bodies);
+     TC.ind_universes := md.(P.ind_universes) |}.
+
+Definition trans_global_decl (d : P.global_decl) : TC.global_decl :=
+  match d with
+  | P.ConstantDecl kn bd => TC.ConstantDecl kn (trans_constant_body bd)
+  | P.InductiveDecl kn bd => TC.InductiveDecl kn (trans_minductive_body bd)
+  end.
+
+Definition trans_global_decls d :=
+  List.map trans_global_decl d.
+
+Definition trans_global (Σ : P.global_env_ext) :=
+  (trans_global_decls (fst Σ), snd Σ).
